use dst-or-subbuffer read to eliminate extra memcpy

src/3d/prelude/buffer/EverParse3d.InputStream.Buffer.fst
@@ -119,11 +119,11 @@ let inst = {
   read = begin fun x n dst ->
     let h0 = HST.get () in
     let currentPosition = !* x.pos in
-    B.blit x.buf currentPosition dst 0ul n;
+    let res = B.sub x.buf currentPosition n in
     x.pos *= currentPosition `U32.add` n;
     let h' = HST.get () in
     assert (B.deref h' x.pos == currentPosition `U32.add` n);
-    ()
+    res
   end;
 
   skip = begin fun x n ->
